RegexCorrectness/NFA/Basic.lean
@@ -4,12 +4,14 @@ import Mathlib.Data.Set.Basic
 
 namespace NFA
 
+/- Returns the set of nodes that can be reached from the given node by consuming the given character. -/
 def Node.charStep (n : Node) (c : Char) : Set Nat :=
   match n with
   | Node.char c' next => if c == c' then {next} else ∅
-  | Node.sparse ranges next => if ranges.any (fun (fst, snd) => c >= fst && c <= snd) then {next} else ∅
+  | Node.sparse ranges next => if ranges.in c then {next} else ∅
   | _ => ∅
 
+/- Returns the set of nodes that can be reached from the given node by consuming ε. -/
 def Node.εStep (n : Node) : Set Nat :=
   match n with
   | Node.epsilon next => {next}
@@ -17,15 +19,17 @@ def Node.εStep (n : Node) : Set Nat :=
   | Node.save _ next => {next}
   | _ => ∅
 
+/- Returns the set of nodes that can be reached from the given node by consuming the given character. -/
 def charStep (nfa : NFA) (i : Nat) (c : Char) : Set Nat :=
-  if h : i < nfa.nodes.size then
-    nfa[i].charStep c
-  else ∅
+  if h : i < nfa.nodes.size
+    then nfa[i].charStep c
+    else ∅
 
+/- Returns the set of nodes that can be reached from the given node by consuming ε. -/
 def εStep (nfa : NFA) (i : Nat) : Set Nat :=
-  if h : i < nfa.nodes.size then
-    nfa[i].εStep
-  else ∅
+  if h : i < nfa.nodes.size
+    then nfa[i].εStep
+    else ∅
 
 theorem charStep_of_charStep {nfa : NFA} {i : Nat} {c : Char} {h : i < nfa.nodes.size}
   (mem : j ∈ nfa[i].charStep c) :
