Regex/Syntax/Hir.lean
@@ -1,38 +1,7 @@
 import Regex.Regex
+import Regex.Intervals
 
 namespace Regex.Syntax.Parser
-
-private def MAX_UNICODE : Nat := 0x10FFFF
-
-private def invertIntervals (int: Array (Char × Char)) : Array (Char × Char) := Id.run do
-  let intervals := int.qsort (λ a b => a.1 < b.1)
-  let mut result := #[]
-  let mut lastEnd : Int := (-1)
-
-  for interval in intervals do
-    let start := interval.1.toNat
-    let end_ := interval.2.toNat
-    if start > lastEnd + 1 then
-      result := result.push (Char.ofNat (lastEnd + 1).toNat, Char.ofNat (start - 1))
-    lastEnd := if end_ > lastEnd then end_ else lastEnd
-
-  if lastEnd < MAX_UNICODE then
-    result := result.push (Char.ofNat (lastEnd + 1).toNat, Char.ofNat MAX_UNICODE)
-
-  return result
-
-private def mergeIntervals (int: Array (Char × Char)) : Array (Char × Char) := Id.run do
-  let intervals := int.qsort (λ a b => a.1 < b.1)
-  let mut merged := #[]
-
-  for interval in intervals do
-    if merged.isEmpty || interval.fst > merged.back.snd then
-      merged := merged.push interval
-    else
-      let snd := Char.ofNat $ Nat.max merged[merged.size-1]!.snd.toNat interval.snd.toNat
-      merged  := merged.set! (merged.size - 1) (merged[merged.size-1]!.fst, snd)
-
-  return merged
 
 inductive PerlClassKind where
   | digit
@@ -40,45 +9,43 @@ inductive PerlClassKind where
   | word
   deriving Repr
 
-def PerlClassKind.toRange : PerlClassKind → Array (Char × Char)
-  | .digit => #[('0', '9')]
-  | .space => #[(' ', ' '), ('\t', '\t'), ('\n', '\n'), ('\r', '\r'), ('\x0B', '\x0B'), ('\x0C', '\x0C')]
-  | .word => #[('a', 'z'), ('A', 'Z'), ('0', '9'), ('_', '_')]
+def PerlClassKind.toRange : PerlClassKind → Intervals
+  | .digit => #[⟨('0', '9'), by decide⟩]
+  | .space => #[⟨(' ', ' '), by decide⟩, ⟨('\t', '\t'), by decide⟩, ⟨('\n', '\n'), by decide⟩, ⟨('\r', '\r'), by decide⟩, ⟨('\x0B', '\x0B'), by decide⟩, ⟨('\x0C', '\x0C'), by decide⟩]
+  | .word => #[⟨('a', 'z'), by decide⟩, ⟨('A', 'Z'), by decide⟩, ⟨('0', '9'), by decide⟩, ⟨('_', '_'), by decide⟩]
 
 structure PerlClass where
   negated: Bool
   kind: PerlClassKind
   deriving Repr
 
-def PerlClass.toRange (perl: PerlClass) : Array (Char × Char) :=
+def PerlClass.toRange (perl: PerlClass) : Intervals :=
   if perl.negated
-    then invertIntervals perl.kind.toRange
+    then Intervals.invert perl.kind.toRange
     else perl.kind.toRange
 
 inductive Interval where
   | single : Char → Interval
-  | range : Char → Char → Interval
+  | range : (s : Char) → (e : Char) → s ≤ e → Interval
   | perl : PerlClass → Interval
-  deriving Repr
 
-def Interval.toRange : Interval → Array (Char × Char)
-  | .single c    => #[(c, c)]
-  | .range c₁ c₂ => #[(c₁, c₂)]
-  | .perl p      => p.toRange
+def Interval.toRange : Interval → Intervals
+  | .single c      => #[⟨(c, c), by simp⟩]
+  | .range c₁ c₂ r => #[⟨(c₁, c₂), r⟩]
+  | .perl p        => p.toRange
 
 structure Classes where
   negated: Bool
   intervals: Array Interval
-  deriving Repr
 
-def Classes.toRange (classes: Classes) : Array (Char × Char) :=
+def Classes.toRange (classes: Classes) : Intervals :=
   let intervals := Array.concatMap (·.toRange) classes.intervals
 
-  let intervals₁ := if classes.negated
-    then invertIntervals intervals
+  let intervals₁ : Intervals := if classes.negated
+    then Intervals.invert intervals
     else intervals
 
-  mergeIntervals intervals₁
+  Intervals.merge intervals₁
 
 inductive Hir : Type where
   | empty : Hir
@@ -91,7 +58,7 @@ inductive Hir : Type where
   | classes : Classes -> Hir
   | perl : PerlClass -> Hir
   | dot : Hir
-deriving Repr, Inhabited
+deriving Inhabited
 
 def Hir.toRegexAux (index : Nat) (hir : Hir) : Nat × Regex :=
   match hir with
@@ -116,7 +83,7 @@ def Hir.toRegexAux (index : Nat) (hir : Hir) : Nat × Regex :=
     (index, .classes c.toRange)
   | .perl p =>
     (index, .classes p.toRange)
-  | .dot => (index, .classes #[(Char.ofNat 0, Char.ofNat MAX_UNICODE)])
+  | .dot => (index, .classes #[⟨(Char.ofNat 0, Char.ofNat Char.MAX_UNICODE), by decide⟩])
 
 def Hir.toRegex (h : Hir) : Regex := (h.toRegexAux 0).2
 
